

Abstract Algebra Herstein - Solutions Manual

Mingruifu Lin

September 2023

Contents

1	Preliminary Notions	5
1.1	Set Theory	5
1.2	Mappings	7
1.3	The Integers	9
2	Group Theory	11
2.1	Some Preliminary Lemmas	11

Chapter 1

Preliminary Notions

1.1 Set Theory

Problem 1

(a) We expand the definitions $A \subseteq B$ and $B \subseteq C$:

$$x \in A \Rightarrow x \in B$$

$$x \in B \Rightarrow x \in C$$

Suppose $x \in A$. Then by modus ponens, $x \in B$. Again by modus ponens, $x \in C$. Hence, by conditional proof, $x \in A \Rightarrow x \in C$. This is the definition of $A \subseteq C$.

(b) Suppose $x \in A \cup B$. We check two cases. If $x \in A$, then $x \in A$. If $x \in B$, then using $B \subseteq A$ and modus ponens, we get $x \in A$, hence $x \in A$. Thus $A \cup B \subseteq A$.

For the reverse direction, suppose $x \in A$. Then $x \in A \cup B$ by disjunction introduction. Thus $A \subseteq A \cup B$. Hence proven.

(c) Too lazy. Disjunctions are always tedious, as seen previously.

Problem 2

(a) For intersection:

$$x \in A \cap B$$

$$\Leftrightarrow x \in A \text{ and } x \in B$$

$$\Leftrightarrow x \in B \cap A$$

For union: Too lazy. Again, too many disjunctions.

(b) Same idea as (a). Simply apply conjunction elimination twice, then conjunction introduction twice.

Problem 3

Here we gooooo.

Suppose $x \in A \cup (B \cap C)$. If $x \in A$, then $x \in A \cup B$ and $x \in A \cup C$, hence $x \in (A \cup B) \cap (A \cup C)$. Otherwise, $x \in B \cap C$, so $x \in B$ and $x \in C$, thus $x \in B \cup A$ and $x \in C \cup A$, hence $x \in (A \cup B) \cap (A \cup C)$. Hence $A \cup (B \cap C) \subseteq (A \cup B) \cap (A \cup C)$.

For the reverse direction, suppose $x \in (A \cup B) \cap (A \cup C)$. Then $x \in A \cup B$ and $x \in A \cup C$. If $x \in A$, then $x \in A \cup (B \cap C)$. If $x \in B$, then, in order to satisfy the second statement, either $x \in A$, which we've seen, or $x \in C$. In the latter case, we thus have $x \in B \cap C$, hence $x \in (B \cap C) \cup A$. In all cases, we have $x \in A \cup (B \cap C)$. Hence $(A \cup B) \cap (A \cup C) \subseteq A \cup (B \cap C)$. Hence proven.

Problem 4

(a)

$$x \in (A \cap B)'$$

$$\Rightarrow x \notin A \cap B$$

Using the fact $\neg(A \wedge B) = \neg A \vee \neg B$:

$$\Rightarrow x \notin A \text{ or } x \notin B$$

$$\Rightarrow x \in A' \text{ or } x \in B'$$

$$\Rightarrow x \in A' \cup B'$$

Too lazy to prove the reverse direction.

(b) Too lazy.

Problem 5

Idk what I'm allowed to do bro.

Problem 6

Include or exclude an element.

Problem 7

At least 39% like both. At most 63% like both.

Problems 8, 9

Too lazy, skipped.

Problem 10

- (a) No. The common ancestor could be different for each pair.
- (b) No. For example, one at far left, one in middle, one at far right.
- (c) Yes.
- (d) Yes.
- (e) No. Equivalence relation must be reflexive.
- (f) Yes.

Problem 11

- (a) The reflexive property guarantees the existence of equivalence classes on non-empty sets, whereas the other properties do not.
- (b) Idk. Maybe $a \in R \Rightarrow a \sim a$.

Problems 12 and 13

Too lazy.

1.2 Mappings**Problem 1**

- (a) Onto, but not one-to-one.
- (b) Both onto and one-to-one. The inverse image is $t\sigma^{-1} = \sqrt{t}$.
- (c) Neither onto nor one-to-one.
- (d) One-to-one, but not onto.

Problem 2

Simply take $f(s \times t) = t \times s$.

Problem 3

Too lazy. Seems obvious.

Problem 4

- (a) Any bijective function has an inverse, which is also a bijection.
- (b) Simply take the composition of the bijection.

Problem 5

???

Problem 6

This is akin to Cantor's diagonal argument. In the original argument, we create a real number which differs from every listed real number by a single digit, hence it is not in the list. Here, the idea is similar.

Suppose I have a bijection $f : S \rightarrow S^*$, where each $s \in S$ is mapped to a subset $f(s) \in S^*$. Let me construct the set $B = \{s \in S \mid s \notin f(s)\}$. In other words, this is the set of elements which are not contained in the subset associated with them. As you see, B differs from $f(s)$ by the single element s for each $f(s)$. If $f(s)$ contains s , then B does not contain s , and if $f(s)$ does not contain s , then B contains s . Since for all bijections f , we can such a set B , hence there exists no bijection between S and S^* .

Problem 7

There are $n!$ ways to permute n objects.

Problem 8

(a) and (b) ??

(c) For (a), as we learned in real analysis, you can map $[0, 1)$ to \mathbb{R} , so you repeat the procedure for every $[n, n + 1)$ for $n \in \mathbb{Z}$. This is onto, but not one-to-one. For (b), simply map \mathbb{R} to $(0, 1)$, which is one-to-one, but not onto.

Problem 9

(a) Using the real numbers again, let $\sigma : \mathbb{R} \rightarrow \mathbb{R}$ and $\tau : (0, 1) \rightarrow \mathbb{R}$, but the range of σ is $(0, 1)$.

(b) Just some domain BS. The first function must be one-to-one, but its range may not cover the entire domain of the second function. So you can do whatever you want to the things outside of the domain.

Problem 10

Classic real analysis exercise. Skipped.

Problem 11

(a) Obvious?

(b) Too easy.

(c) Again, domain BS.

Problem 12

??

Problem 13

- (a) Let $\sigma : n \mapsto 2n$.
 (b) Let $\sigma : \mathbb{R} \rightarrow (0, 1)$, which is easily found if you know real analysis.
 (c) A is infinite, so it has a map $f : A \rightarrow a$, where $a \subset A$. Then, we use the identity function on $S \setminus A$. Combining the two functions, we effectively get a bijection $g : S \rightarrow s$ where $s \subset S$:

$$g(x) = \begin{cases} f(x) & x \in A \\ i(x) & x \in S \setminus A \end{cases}$$

Problem 14

Classic exercise in real analysis.

Problems 15 and 16

Obvious.

1.3 The Integers**Problem 1**

$$\begin{aligned} a \mid b &\Rightarrow b = k_1 a \\ b \mid a &\Rightarrow a = k_2 b \end{aligned}$$

Where k_1, k_2 are integers. But we know $k_2 = \frac{1}{k_1}$, and in order for k_2 to remain an integer, k_1 must be equal to 1 or -1 (this can be proved by induction). Hence, $b = (\pm 1)a = \pm a$.

Problem 2

$$b \mid g, \quad b \mid h \quad \Rightarrow \quad b \mid mg, \quad b \mid nh \quad \Rightarrow \quad b \mid mg + nh$$

Problem 3

Let $d = \frac{ab}{(a,b)} = \frac{a}{(a,b)}b$. Since $(a,b) \mid a$, then $\frac{a}{(a,b)}$ is an integer, hence $b \mid d$. The same procedure can be done for $a \mid d$. Hence, d satisfies the first property.

For the second property, first note that if $a = m(a,b)$ and $b = n(a,b)$, then $(m,n) = 1$. Suppose for contradiction that $k \mid m$ and $k \mid n$ for some $k > 1$. Then

$$k(a,b) \mid m(a,b) = a$$

and

$$k(a,b) \mid n(a,b) = b$$

hence $k(a,b) \mid a, b$ but $k(a,b) \nmid (a,b)$, contradicting the fact that (a,b) is the GCD. Hence $(m,n) = 1$.

SKIP.

Problem 4

$$am = bn$$

Since $(a, b) = 1$, and $a \mid bn$, then $a \mid n$. Hence $ab \mid nb = x$.

Problem 5

(a) Obviously, $p_1^{\delta_1} \dots p_k^{\delta_k}$ divides both a and b . Now, suppose $x \mid a, b$. We can develop its prime factorization. So $x = p_1^{\omega_1} \dots p_k^{\omega_k} \mid a, b$. Which means $p_i^{\omega_i} \mid a, b$, for each i . But $p_i^{\omega_i}$ is coprime with every other prime of a, b , so it must divide the non-coprime part, which only consists of the prime equal to him, hence $p_i^{\omega_i} \mid p_i^{\alpha_i}$ and $p_i^{\omega_i} \mid p_i^{\beta_i}$. Hence, it must divide the minimum power, so $\omega_i \mid \min(\alpha_i, \beta_i) = p_i^{\delta_i}$. Multiplying every $p_i^{\omega_i}$ together, we get $p_1^{\omega_1} \dots p_k^{\omega_k} \mid p_1^{\delta_1} \dots p_k^{\delta_k}$, which gives us our desired result.

(b) We use the formula proven in Problem 3.

$$[a, b] = \frac{ab}{(a, b)}$$

Let's concentrate on a single prime at a time. For prime i , we have

$$\begin{aligned} p_i^{\gamma_i} &= \frac{p_i^{\alpha_i} p_i^{\beta_i}}{p_i^{\min(\alpha_i, \beta_i)}} \\ &= p_i^{\alpha_i + \beta_i - \min(\alpha_i, \beta_i)} \\ &= p_i^{\max(\alpha_i, \beta_i)} \end{aligned}$$

Problem 6

Proof by induction. Base case. r_{n-1} is divisible by r_n .

$$r_{n-1} = q_n r_n + r_{n+1} = q_n r_n + 0 = q_n r_n$$

And obviously, r_n is divisible by r_n .

Now, suppose r_{k-1} and r_k are divisible by r_k , then

$$r_{k-2} = q_{k-1} r_{k-1} + r_k$$

indicates that r_{k-2} is obviously divisible by r_k . Here, we thus proved:

$$r_k \mid r_k \text{ and } r_k \mid r_{k-1} \Rightarrow r_k \mid r_{k-1} \text{ and } r_k \mid r_{k-2}$$

which completes our induction step. (a and b are precisely $r_{(-1)}$ and r_0 .)

Chapter 2

Group Theory

2.1 Some Preliminary Lemmas

Problem 1

- (a) No. Not associative
- (b) No. Missing inverse.
- (c) Yes.
- (d) Yes.

Problem 2

Just repeatedly swap.

Problem 3

For all a, b , we have

$$(a \cdot b)^2 = a^2 \cdot b^2$$

$$a \cdot b \cdot a \cdot b = a \cdot a \cdot b \cdot b$$

Take inverse on each end.

$$\Rightarrow b \cdot a = a \cdot b$$

Problem 4

We are given (1)

$$(ab)^i = a^i b^i$$

and (2)

$$(ab)^{i+1} = a^{i+1} b^{i+1}$$

$$\Rightarrow (ba)^i = a^i b^i$$

and (3)

$$\begin{aligned}(ab)^{i+2} &= a^{i+2}b^{i+2} \\ \Rightarrow (ba)^{i+1} &= a^{i+1}b^{i+1}\end{aligned}$$

We substitute (2) into (3), then regroup, giving the result (4)

$$\begin{aligned}\Rightarrow (ba)^{i+1} &= a(ba)^ib \\ \Rightarrow ba(ba)^i &= ab(ab)^i\end{aligned}$$

Notice that we can equate a^ib^i in (1) and (2), giving the result (5)

$$(ab)^i = a^ib^i = (ba)^i$$

Now, we substitute (5) into (4), which becomes

$$\Rightarrow ba(ba)^i = ab(ba)^i$$

Taking the inverse on each side gives the desired result.

Problem 5

??

Problem 6

Let $x = 1 \leftrightarrow 2$. Let $y = 2 \leftrightarrow 3$. Then $(xy)^2$ will cause $123 \rightarrow 312$, while x^2y^2 would be identity $123 \rightarrow 123$.

Problem 7

The identity operation, as well as the 2-element swaps, satisfy $x^2 = e$. The 3-element cycles satisfy $x^3 = e$. It's then easy to count.

Problem 8

Suppose for contradiction that $a^N \neq e$ for all $N \in \mathbb{N}$. We show that this implies $a^X \neq a^Y$ for all pairs $X \neq Y$. Suppose for (nested) contradiction that $a^X = a^Y$ for some pair $X > Y > 1$. Then taking the inverse on both sides yields $a^{X-Y} = e$, contradicting the fact that $a^N \neq e$ for all N . Hence, $a^X \neq a^Y$, i.e. the powers of a are pairwise distinct. However, we know our group is finite, but a^N creates infinite distinct elements. Hence, it must be false, so $a^N = e$ for some N .

Problem 9

(a)

$$G = \{e, x, y\}$$

Since identity e is unique, then $xy \neq x$. Because, otherwise, we would have $y = e$, which is false. Similarly, $xy \neq y$. So, using the fact that groups are closed, xy must have some result in G , the only one left being $xy = e$. Property of inverse implies that $yx = e$ as well. Hence x commutes with y . Finally, we know the identity commutes with every elements. Hence proven.

(b)

$$G = \{e, x, y, z\}$$

Suppose $xy = yx = e$, then xz cannot equal x nor z , because neither is equal to the unique e . It also cannot equal e , because x, y are already inverse pairs, and inverses are unique, so z cannot be another inverse. Hence xz can only equal y , by the closure property. This procedure is repeated for zx, yz, zy , which must equal y, x, x respectively. Hence, $xy = yx = e$ and $xz = zx = y$ and $yz = zy = x$, where e already commutes with everyone.

Now, suppose $x^2 = e$ and $y^2 = e$. Since inverses are unique, we have $z^2 = e$. And thus $xy = yx = z$ and $xz = zx = y$ and $yz = zy = x$ (same logic as before, none can be identity, and none is inverse pair). And e already commutes with everyone.

All cases have been gone over. Hence proven.

(c) Too lazy. We know every group of prime order must be cyclic, therefore abelian.

Problem 10

For every pair x, y , we have

$$\begin{aligned} (xy)^2 &= e = ee = x^2y^2 \\ &\Rightarrow xyxy = xxyy \end{aligned}$$

Taking inverse on both extremities of each side yields

$$yx = xy$$

Problem 11

Inverses come in pairs. But e is paired with itself. So if the group order is even, then there is an odd number of non- e elements. Hence, another element must be paired with itself.

Problem 12